\documentclass[a4paper]{article}

\usepackage{setup}

\hypersetup{pdfstartview=XYZ}%         zoom par defaut

\setlength{\droptitle}{-5em}   % This is your set screw
\title{\vspace{1.5cm}Declarative type system}
\author{}
\date{\vspace{-5ex}}

\pagenumbering{gobble}

\theoremstyle{definition}
\newtheorem{theorem}{Theorem}
\newtheorem{lemma}{Lemma}
\newtheorem{definition}{Definition}
\newtheorem{property}{Property}
\newtheorem{corollary}{Corollary}

\begin{document}

  \maketitle
  
    \section{Typing rules}

    TODO: make $\cvdash p e t$ operate on environment instead of expression? May be more intuitive...

    \begin{mathpar}
      \Infer[Occ]
          { }
          { \Gamma \vdash e: \Gamma(e) }
          { e\in\dom\Gamma }
      \qquad
      \Infer[Intersect]
          { \Gamma \vdash e:t_1\\\Gamma \vdash e:t_2 }
          { \Gamma \vdash e: t_1 \wedge t_2 }
          { }
      \qquad
      \Infer[Subs]
          { \Gamma \vdash e:t\\t\leq t' }
          { \Gamma \vdash e: t' }
          { }
      \qquad
      \\
      \Infer[Const]
          { }
          {\Gamma\vdash c:\basic{c}}
          { }
      \qquad
      \Infer[App]
          {
            \Gamma \vdash e_1: \arrow {t_1}{t_2}\\
            \Gamma \vdash e_2: t_1
          }
          { \Gamma \vdash {e_1}{e_2}: t_2 }
          { }
          \\
      \Infer[Abs]
          {\Gamma,x:s_i\vdash e:t_i\\t\simeq \left(\bigwedge_{i\in I} \arrow {s_i} {t_i}\right)
          \land \left(\bigwedge_{j\in J} \neg (\arrow {s'_j} {t'_j})\right)\\t\not\simeq\Empty}
          {
          \Gamma\vdash\lambda^{\wedge_{i\in I}\arrow {s_i} {t_i}}x.e:\textstyle t
          }
          { }
          \\
      \Infer[If]
            {\Gamma\vdash e:t_0\\
            t_0\not\leq \neg t \Rightarrow
            \Gamma \cvdash + e t e_1:t'\\
            t_0\not\leq t \Rightarrow
            \Gamma \cvdash - e t e_2:t'}
            {\Gamma\vdash \ite {e} t {e_1}{e_2}: t'}
            { }
      \qquad
      \Infer[Empty]
      { }
      { \Gamma, (e:\Empty) \vdash e': \Empty }
      { }
      \\
      \Infer[Proj]
      {\Gamma \vdash e:(t_1,t_2)}
      {\Gamma \vdash \pi_i e:t_i}
      { }
      \qquad
      \Infer[Pair]
      {\Gamma \vdash e_1:t_1 \and \Gamma \vdash e_2:t_2}
      {\Gamma \vdash (e_1,e_2):\pair {t_1} {t_2}}
      { }
    \end{mathpar}

    \begin{center} \line(1,0){450} \end{center}

    \begin{mathpar}
      \Infer[Base]
          { \Gamma \vdash e':t' }
          { \Gamma \cvdash p e t e':t' }
          { }
          \qquad
      \Infer[Path]
          { \pvdash \Gamma p e t \varpi:t_1 \\ \Gamma,(\occ e \varpi:t_1) \cvdash p e t e':t_2 }
          { \Gamma \cvdash p e t e':t_2 }
          { }
    \end{mathpar}

    \begin{center} \line(1,0){450} \end{center}

    \begin{mathpar}
      \Infer[PTypeof]
          { \Gamma \vdash \occ e \varpi:t' }
          { \pvdash \Gamma p e t \varpi:t' }
          { }
          \qquad
      \Infer[PIntersect]
          { \pvdash \Gamma p e t \varpi:t_1 \\ \pvdash \Gamma p e t \varpi:t_2 }
          { \pvdash \Gamma p e t \varpi:t_1\land t_2 }
          { }
          \qquad
      \Infer[PSubs]
          { \pvdash \Gamma p e t \varpi:t_1 \\ t_1\leq t_2 }
          { \pvdash \Gamma p e t \varpi:t_2 }
          { }
          \\
      \Infer[PEps+]
          { }
          { \pvdash \Gamma + e t \epsilon:t }
          { }
          \qquad
      \Infer[PEps-]
          { }
          { \pvdash \Gamma - e t \epsilon:\neg t }
          { }
          \\
      \Infer[PAppL]
          { \pvdash \Gamma p e t \varpi.1:t_1 \\ \pvdash \Gamma p e t \varpi:t_2 }
          { \pvdash \Gamma p e t \varpi.0:\neg (\arrow {t_1} {\neg t_2}) }
          { }
          \qquad
      \Infer[PAppR]
          { \pvdash \Gamma p e t \varpi.0:\arrow{t_1}{t_2} \\ \pvdash \Gamma p e t \varpi:t_2' \\ t_2\land t_2' \simeq \Empty }
          { \pvdash \Gamma p e t \varpi.1:\neg t_1 }
          { }
          \\
      \Infer[PPairL]
          { \pvdash \Gamma p e t \varpi:\pair{t_1}{t_2} }
          { \pvdash \Gamma p e t \varpi.l:t_1 }
          { }
          \qquad
      \Infer[PPairR]
          { \pvdash \Gamma p e t \varpi:\pair{t_1}{t_2} }
          { \pvdash \Gamma p e t \varpi.r:t_2 }
          { }
          \qquad
      \Infer[PFst]
          { \pvdash \Gamma p e t \varpi:t' }
          { \pvdash \Gamma p e t \varpi.f:\pair {t'} \Any }
          { }
          \qquad
      \Infer[PSnd]
          { \pvdash \Gamma p e t \varpi:t' }
          { \pvdash \Gamma p e t \varpi.s:\pair \Any {t'} }
          { }
          \qquad
    \end{mathpar}

    \newpage

    \section{Intermediate semantics}

    \[
      \begin{array}{lrcl}
      \textbf{Expressions} & e & ::= & c\alt x \alt \lambda^{\bigwedge \arrow t t}x.e \alt e e \alt \ite e t e e\\
      \textbf{Values} & v & ::= & c \alt \lambda^{\bigwedge \arrow t t}x.e
      \end{array}
    \]

    \[
      \begin{array}{lrcl}
      \textbf{Context} & C[] & ::= & e [] \alt [] v
      \end{array}
    \]

    For convenience, we denote $e\xleadsto{e\mapsto e'}e'$ by $e\idleadsto e'$.

    \begin{mathpar}
      \Infer[Ctx]
      {e \xleadsto{e_r\mapsto e_r'} e'}
      {C[e] \xleadsto{e_r\mapsto e_r'} C[e']}
      {}
      \qquad
      \Infer[App]
      { }
      {(\lambda^tx.e) v \idleadsto e\subst x v}
      {}\\
      \Infer[TestCtx]
      {e \xleadsto{e_r\mapsto e_r'} e'}
      {\ite e t {e_1} {e_2} \idleadsto \ite {e'} t {e_1\subst {e_r} {e_r'}} {e_2\subst {e_r} {e_r'}}}
      {}\\
      \Infer[Ite]
      {i \in \{1,2\}\hspace{1cm} (i=1 \Leftrightarrow v \in \valsemantic t)}
      {\ite v t {e_1} {e_2} \idleadsto e_i}
      {}
    \end{mathpar}

    \[\valsemantic t = \{v \alt \vvdash v : t\}\]

    \begin{mathpar}
      \Infer[Subsum]
          {\vvdash v:t'\\t'\leq t}
          {\vvdash v:t}
          {}
      \qquad
      \Infer[Const]
          { }
          {\vvdash c:\basic{c}}
          {}
      \\
      \Infer[Abs]
          {t=(\wedge_{i\in I}\arrow {s_i} {t_i})\land (\wedge_{j\in J} \neg (\arrow {s'_j} {t'_j}))\\t\not\leq \Empty}
          {\vvdash\lambda^{\wedge_{i\in I}\arrow {s_i} {t_i}}x.e:t}
          {}
      \\
      \end{mathpar}

\end{document}